\documentclass{lecturenotes}

\usepackage[colorlinks,urlcolor=blue]{hyperref}
\usepackage{doi}
\usepackage{xspace}
\usepackage{agda}
\usepackage{fontspec}
\usepackage{enumerate}
\usepackage{amsmath}
\setsansfont{Fira Code}
\usepackage{newunicodechar}
\newunicodechar{∣}{\ensuremath{\mid}}
\newunicodechar{′}{\ensuremath{{}^\prime}}
\newunicodechar{⊎}{\ensuremath{\uplus}}
\newunicodechar{₁}{\ensuremath{{}_1}}
\newunicodechar{₂}{\ensuremath{{}_2}}

\newcommand{\agdanats}{\textsf{ℕ}\xspace}
\newcommand{\agdaempty}{\textsf{⊥}\xspace}

\title{Negation}
\coursenumber{CSE 410/510}
\coursename{Programming Language Theory}
\lecturenumber{7}
\semester{Spring 2025}
\professor{Professor Andrew K. Hirsch}

\begin{document}
\maketitle

\begin{code}
module lec07 where

open import Relation.Binary.PropositionalEquality using (_≡_; refl)
open import Data.Nat using (ℕ; zero; suc)
open import Data.Empty using (⊥; ⊥-elim)
open import Data.Sum using (_⊎_; inj₁; inj₂)

postulate
  extensionality : ∀ {A B : Set} {f g : A → B}
    → (∀ (x : A) → f x ≡ g x)
    -------------------------
    → f ≡ g
\end{code}

\section{Negation}
\label{sec:neg}

\begin{itemize}
\item Negation key-binding in Agda-mode is \texttt{\textbackslash lnot}. 
\item We can define negation as follows:
\begin{code}
¬_ : Set → Set
¬ A = A → ⊥
\end{code}
\item Here, \texttt{\lnot} is a function that takes a proposition \texttt{A} and returns a \agdaempty.
\item Because there is no way to construct an impossible promise \agdaempty, this means that \texttt{A} cannot be true.

\item If we have evidence for both \texttt{\lnot A} and \texttt{A}, we can derive a contradiction:
\begin{code}
¬-elim : ∀ {A : Set}
    → ¬ A
    → A
    --------
    → ⊥
¬-elim fx x = fx x
\end{code}
\item We can prove this by applying \texttt{fx} to \texttt{x}, which gives us \agdaempty.
      This is returning something impossible by combining something impossible we received together.

\item The previous example is \textbf{not an example of proof by contradiction}.
      A proof by contradiction proves \texttt{P} by assuming \texttt{\lnot P} and then deriving a contradiction. 
      A direct proof of \texttt{\sim P} is just a direct proof of \texttt{P -> False}: assume \texttt{P} and derive false.

\item If we have evidence for \texttt{A}, it implies \texttt{\lnot \lnot A}:
\begin{code}
¬¬-intro : ∀ {A : Set}
    → A
    --------
    → ¬ ¬ A
¬¬-intro a = λ {¬a → ¬a a}

-- ¬ ¬ A → A
\end{code}
\item Here, \texttt{a} is evidence of \texttt{A} we provide. We also have a lambda function that 
      takes \texttt{¬a} and returns \texttt{¬a a} which is \agdaempty. And we take that as evidence for \texttt{\lnot A}. 
      Now we have \texttt{A} and \texttt{\lnot A}, which is impossible. Therefore, we have \texttt{\lnot \lnot A}.
\item \textbf{But we cannot prove \texttt{A} from \texttt{\lnot \lnot A} in Agda}, we will discuss it later on.

\item We can negate the bottom:
\begin{code}
id-⊥ : ¬ ⊥ 
id-⊥ = λ {x → x}
\end{code}
\item If we receive evidence for \agdaempty, we just return it. 
      So \texttt{\lnot \agdaempty} is equivalent to \texttt{\agdaempty \rightarrow \agdaempty}.

\item Another way to do this is using pattern matching:
\begin{code}
id-⊥′ : ⊥ → ⊥
id-⊥′ ()
\end{code}
\item Since \agdaempty does not have any constructors, so there's no possible pattern match.

\item Extensionality means that if two functions are pointwise equal, then they are equal.
      Since we don't have constructors for \agdaempty, there is no element in their domains,
      we can obviously use extensionality to prove that they are equal:
\begin{code}
id≡id′ : id-⊥ ≡ id-⊥′
id≡id′ = extensionality (λ())
\end{code}

\item Any proofs of a negation are equal:
\begin{code}
assimilation : ∀ {A : Set} (¬x ¬y : ¬ A) → ¬x ≡ ¬y
assimilation ¬x ¬y = extensionality (λ x → ⊥-elim (¬x x))
\end{code}

\item We can define inequality by negating equality:
\begin{code}
_≢_ : ∀ {A : Set} → A → A → Set
x ≢ y = ¬ (x ≡ y)

_ : 1 ≢ 2
_ = λ ()
\end{code}
\item Agda has the property that objects of different constructors will never be the same.
      In \agdanats, since \texttt{zero} is not the successor of anything, we can prove that:

\begin{code}
peano : ∀ {m : ℕ} → zero ≢ suc m
peano = λ () -- There is no possible pattern for m s.t. zero is equal to suc m
\end{code}
\end{itemize} % End of Section 1

\section{Intuitionistic Logic}
\label{sec:intui-logic}

\begin{itemize}
\item Previously, we have seen that \texttt{\lnot \lnot A} does not imply \texttt{A} in Agda.
\item This is because Agda is an \textbf{intuitionistic logic} system. 
      In intuitionistic logic, we cannot prove a proposition is true by proving that its negation is false.
      Therefore, given a double negation, we cannot conclude that the proposition is true.
\item In proof by contradiction, we have a goal \texttt{P}, we first assume \texttt{\lnot P} and derive \agdaempty.
      Then we can conclude that \texttt{P} holds. When \texttt{\lnot P} leads to \agdaempty, it is the same as 
      \texttt{\lnot \lnot P}, and it does not implies \texttt{P}. Therefore, for similar reason, proof by contradiction is not supported in Agda.

\item But trible-negation can implies negation:
\begin{code}
¬¬¬-intro : ∀ {A : Set}
    → ¬ ¬ ¬ A
    --------
    → ¬ A
¬¬¬-intro ¬¬¬x x = ¬¬¬x (¬¬-intro x)
\end{code}
\item Here, we assume \texttt{x} is an evidence for \texttt{A}. We can use \texttt{¬¬-intro} with \texttt{x} to prove \texttt{\lnot \lnot A},
      and then we use this result as an argument for \texttt{¬¬¬x}, which gives us a contradiction.
      So if we assume \texttt{A} is true and it leads to a contradiction, we can conclude that \texttt{\lnot A} is true.

\item Another srike system of intuitionistic logic system or Agda, is that
      \textbf{we cannot prove the law of excluded middle}:
\begin{code}
postulate
  lem : ∀ {A : Set} →  A ⊎ ¬ A
\end{code}
\item As we discussed before, we cannot prove a proposition is true by proving that its negation is false.

\item But, we can show that \textbf{law of excluded middle is irrefutable}:
\begin{code}
lem-irrefutable : ∀ {A : Set} → ¬ ¬ (A ⊎ ¬ A)
lem-irrefutable k = k (inj₂ (λ x → k (inj₁ x)))
\end{code}

\begin{enumerate}
\item At the beginning when we build the proof of \texttt{lem-irrefutable},
      we have an evidence \texttt{k} that leads to \texttt{\lnot (A \uplus \lnot A)}:
      \\ \texttt{lem-irrefutable k = \{!!\} -- Goal : \agdaempty}

\item The evidence \texttt{k} is a function that given a value of type \texttt{A \uplus \lnot A},
      returns \agdaempty. So we apply \texttt{k} to the hole to get a goal of \agdaempty :
      \\ \texttt{lem-irrefutable k = k \{!!\} -- Goal : lem A} 

\item The goal of the hole now becomes \texttt{lem}. Since we have no evidence of \texttt{A},
      we start from the right side, and assume \texttt{\lnot A}:
      \\ \texttt{lem-irrefutable k = k (inj₂ (\lambda\ x → \{!!\})) -- Goal : \agdaempty}

\item The second disjunct of \texttt{lem} accepts evidence \texttt{\lnot A}, in this lambda function, we bind \texttt{x}
      to \texttt{A}, and return \agdaempty. Again, we apply \texttt{k} to the hole to get a goal of \agdaempty :
      \\ \texttt{lem-irrefutable k = k (inj₂ (\lambda\ x → k \{!!\})) -- Goal : lem A}

\item The goal of the hole is again \texttt{lem}, but this time we have the evidence of \texttt{A},
      so we go to the left side, assume \texttt{A} and give it \texttt{x}:
      \\ \texttt{lem-irrefutable k = k (inj₂ (\lambda\ x → k (inj₁ x))) -- no hole left}
\end{enumerate}
\end{itemize} % End of Section 2

\end{document}

%%% Local Variables:
%%% mode: latex
%%% TeX-master: t
%%% TeX-engine: luatex
%%% TeX-command-default: "Make"
%%% End:
